AwsCryptographicMaterialProviders/dafny/AwsCryptographyKeyStore/src/CreateKeys.dfy
@@ -37,7 +37,7 @@ module CreateKeys {
   // A GenerateDataKeyWithoutPlaintext of request size 32 returns a ciphertext size of 184 bytes.
   const KMS_GEN_KEY_NO_PLAINTEXT_LENGTH_32 := 184;
 
-  type branchKeyItem = m: map<string, string> | branchKeyContextHasRequiredFields?(m) witness *
+  type BranchKeyContext = m: map<string, string> | branchKeyContextHasRequiredFields?(m) witness *
   predicate method branchKeyContextHasRequiredFields?(m: map<string, string>) {
     && KEY_IDENTIFIER_FIELD in m
     && TYPE_FIELD in m
@@ -55,6 +55,20 @@ module CreateKeys {
       KEY_IDENTIFIER_FIELD := id,
       TYPE_FIELD := BRANCH_KEY_TYPE_PREFIX + version,
       KEY_STATUS := "ACTIVE",
+      KEY_CREATE_TIME := timestamp,
+      TABLE_FIELD := tableName,
+      KMS_FIELD := kmsKeyArn,
+      HIERARCHY_VERSION := "1"
+    ]
+  }
+
+  function method decryptOnlyBranchKeyEncryptionContext(id: string, version: string, timestamp: string, tableName: string, kmsKeyArn: string): (output: map<string, string>)
+    ensures branchKeyContextHasRequiredFields?(output)
+  {
+    map[
+      KEY_IDENTIFIER_FIELD := id,
+      TYPE_FIELD := BRANCH_KEY_TYPE_PREFIX + version,
+      KEY_STATUS := "DECRYPT_ONLY",
       KEY_CREATE_TIME := timestamp,
       TABLE_FIELD := tableName,
       KMS_FIELD := kmsKeyArn,
@@ -85,8 +99,13 @@ module CreateKeys {
     ensures ddbClient.ValidState() && kmsClient.ValidState()
   {
     var maybeBranchKeyId := UUID.GenerateUUID();
+    //= aws-encryption-sdk-specification/framework/branch-key-store.md#branch-key-and-beacon-key-creation
+    //# - `branchKeyId`: a new guid. This guid MUST be [version 4 UUID](https://www.ietf.org/rfc/rfc4122.txt)
     var branchKeyId :- maybeBranchKeyId
       .MapFailure(e => Types.KeyStoreException(message := e));
+    //= aws-encryption-sdk-specification/framework/branch-key-store.md#branch-key-and-beacon-key-creation
+    //# - `timestamp`: a timestamp for the current time. 
+    //# This MUST be in ISO8601 format in UTC, to microsecond precision (e.g. “YYYY-MM-DDTHH:mm:ss.ssssssZ“)
     var timestamp :- Time.GetCurrentTimeStamp()
       .MapFailure(e => E(e));
 
@@ -98,12 +117,9 @@ module CreateKeys {
       E("CreateKey received invalid grant tokens")
     );
     
-    //= aws-encryption-sdk-specification/framework/branch-key-store.md#createkey
-    //# This operation MUST create both a [branch key](#branch-key) and a [beacon key](#beacon-key) according to
-    //# the [Branch Key and Beacon Key Creation](#branch-key-and-beacon-key-creation) section.
-    
-    // Branch Key Creation
     var maybeBranchKeyVersion := UUID.GenerateUUID();
+    //= aws-encryption-sdk-specification/framework/branch-key-store.md#branch-key-and-beacon-key-creation
+    //# - `version`: a new guid. This guid MUST be [version 4 UUID](https://www.ietf.org/rfc/rfc4122.txt)
     var branchKeyVersion :- maybeBranchKeyVersion
       .MapFailure(e => Types.KeyStoreException(message := e));
 
@@ -113,9 +129,14 @@ module CreateKeys {
       Types.KeyStoreException(message := "Failed to generate UUID for Key ID or Key Version.")
     );
     
-    var activeBranchKeyEncryptionContext: branchKeyItem := activeBranchKeyEncryptionContext(branchKeyId, branchKeyVersion, timestamp, ddbTableName, kmsKeyArn);
+    var activeBranchKeyEncryptionContext: BranchKeyContext := activeBranchKeyEncryptionContext(branchKeyId, branchKeyVersion, timestamp, ddbTableName, kmsKeyArn);
 
+    //= aws-encryption-sdk-specification/framework/branch-key-store.md#branch-key-and-beacon-key-creation
+    //# The operation MUST call [AWS KMS API GenerateDataKeyWithoutPlaintext]
+    //# (https://docs.aws.amazon.com/kms/latest/APIReference/API_GenerateDataKeyWithoutPlaintext.html).
     var branchKeyWithoutPlaintext :- GenerateKey(
+      //= aws-encryption-sdk-specification/framework/branch-key-store.md#branch-key-and-beacon-key-creation
+      //# - `EncryptionContext` MUST be the [encryption context for branch keys](#encryption-context).
       activeBranchKeyEncryptionContext,
       kmsKeyArn,
       grantTokens.value,
@@ -123,15 +144,24 @@ module CreateKeys {
     );
 
     // Beacon Key Creation
-    var beaconKeyEncryptionContext: branchKeyItem := beaconKeyEncryptionContext(branchKeyId, timestamp, ddbTableName, kmsKeyArn);
+    var beaconKeyEncryptionContext: BranchKeyContext := beaconKeyEncryptionContext(branchKeyId, timestamp, ddbTableName, kmsKeyArn);
 
+    //= aws-encryption-sdk-specification/framework/branch-key-store.md#branch-key-and-beacon-key-creation
+    //# The operation MUST call [AWS KMS API GenerateDataKeyWithoutPlaintext]
+    //# (https://docs.aws.amazon.com/kms/latest/APIReference/API_GenerateDataKeyWithoutPlaintext.html).
     var beaconKeyWithoutPlaintext :- GenerateKey(
+      //= aws-encryption-sdk-specification/framework/branch-key-store.md#branch-key-and-beacon-key-creation
+      //# - `EncryptionContext` MUST be the [encryption context for beacon keys](#encryption-context).
       beaconKeyEncryptionContext,
       kmsKeyArn,
       grantTokens.value,
       kmsClient
     );
 
+    //= aws-encryption-sdk-specification/framework/branch-key-store.md#createkey
+    //# If creation of both keys is successful, 
+    //# this operation MUST call [Amazon DynamoDB API TransactWriteItems]
+    //# (https://docs.aws.amazon.com/amazondynamodb/latest/APIReference/API_TransactWriteItems.html).
     var transactWriteItemsToKeyStore :- WriteNewKeyToStore(
       activeBranchKeyEncryptionContext,
       branchKeyWithoutPlaintext.CiphertextBlob.value,
@@ -141,6 +171,9 @@ module CreateKeys {
       ddbClient
     );
 
+    //= aws-encryption-sdk-specification/framework/branch-key-store.md#createkey
+    //# If writing to the key store succeeds, the operation MUST return the branch-key-id that maps to both
+    //# the branch key and the beacon key.
     res := Success(Types.CreateKeyOutput(
       branchKeyIdentifier := branchKeyId 
     ));
@@ -209,9 +242,9 @@ module CreateKeys {
   }
 
   method WriteNewKeyToStore(
-    branchKeyItem: branchKeyItem,
+    branchKeyContext: BranchKeyContext,
     wrappedBranchKey: seq<uint8>,
-    beaconKeyItem: branchKeyItem,
+    beaconKeyContext: BranchKeyContext,
     wrappedBeaconKey: seq<uint8>,
     tableName: DDB.TableName,
     ddbClient: DDB.IDynamoDBClient
@@ -221,10 +254,10 @@ module CreateKeys {
     modifies ddbClient.Modifies
     ensures ddbClient.ValidState()
   {
-    var branchKeyDDBMap := ToBranchKeyItemAttributeMap(branchKeyItem, wrappedBranchKey);
+    var branchKeyDDBMap := ToBranchKeyItemAttributeMap(branchKeyContext, wrappedBranchKey);
     var branchKeyTransactWriteItem := CreateTransactWritePutItem(branchKeyDDBMap, tableName);
 
-    var beaconKeyDDBMap := ToBranchKeyItemAttributeMap(beaconKeyItem, wrappedBeaconKey);
+    var beaconKeyDDBMap := ToBranchKeyItemAttributeMap(beaconKeyContext, wrappedBeaconKey);
     var beaconKeyTransactWriteItem := CreateTransactWritePutItem(beaconKeyDDBMap, tableName);
     
     :- Need(
@@ -254,7 +287,50 @@ module CreateKeys {
     res := Success(transactWriteItemsResponse);
   }
 
-  function method ToBranchKeyItemAttributeMap(m: branchKeyItem, k: seq<uint8>): (output: DDB.AttributeMap)
+  method WriteVersionedKeyToStore(
+    decryptOnlyBranchKey: DDB.AttributeMap,
+    newActiveBranchKey: DDB.AttributeMap,
+    tableName: DDB.TableName,
+    ddbClient: DDB.IDynamoDBClient
+  )
+    returns (res: Result<DDB.TransactWriteItemsOutput, Types.Error>)
+    requires ddbClient.ValidState()
+    modifies ddbClient.Modifies
+    ensures ddbClient.ValidState()
+  {
+    var decryptOnlyBranchKeyTransactWriteItem := CreateTransactWritePutItem(decryptOnlyBranchKey, tableName);
+    var newActiveBranchKeyTransactWriteItem := CreateTransactWritePutItem(newActiveBranchKey, tableName);
+
+    :- Need(
+      // In order to be certain we are writing something that is well formed
+      // and something we will be able to get or query we need to ensure it has certain properties
+      && validActiveBranchKey?(newActiveBranchKey)
+      && validVersionBranchKey?(decryptOnlyBranchKey),
+      Types.KeyStoreException(message := "Unable to write key material to Key Store: " + tableName)
+    );
+
+    var items: DDB.TransactWriteItemList := [
+      decryptOnlyBranchKeyTransactWriteItem,
+      newActiveBranchKeyTransactWriteItem 
+    ];
+    
+    var transactRequest := DDB.TransactWriteItemsInput(
+      TransactItems := items,
+      ReturnConsumedCapacity := None,
+      ReturnItemCollectionMetrics := None,
+      ClientRequestToken := None
+    );
+    
+    var maybeTransactWriteResponse := ddbClient.TransactWriteItems(transactRequest);
+    var transactWriteItemsResponse :- maybeTransactWriteResponse
+      .MapFailure(e => Types.ComAmazonawsDynamodb(ComAmazonawsDynamodb := e));
+
+    res := Success(transactWriteItemsResponse);
+  }
+
+  // We specify that every item on the encryption context to KMS is stored in the branch/beacon key item.
+  // This method allows us to convert from a BranchKeyContext map to a DDB.AttributeMap easily.
+  function method ToBranchKeyItemAttributeMap(m: BranchKeyContext, k: seq<uint8>): (output: DDB.AttributeMap)
   {
     map[
       KEY_IDENTIFIER_FIELD := DDB.AttributeValue.S(m[KEY_IDENTIFIER_FIELD]),
@@ -283,9 +359,306 @@ module CreateKeys {
     )
   }
 
-  method VersionActiveBranchKey(input: Types.VersionKeyInput, ddbTableName: DDB.TableName, kmsClient: KMS.IKMSClient, ddbClient: DDB.IDynamoDBClient)
+  method VersionActiveBranchKey(input: Types.VersionKeyInput, ddbTableName: DDB.TableName, kmsKeyArn: Types.KmsKeyArn, kmsClient: KMS.IKMSClient, ddbClient: DDB.IDynamoDBClient)
     returns (res: Result<(), Types.Error>)
+    requires KMS.IsValid_KeyIdType(kmsKeyArn)
+    requires ddbClient.ValidState() && kmsClient.ValidState()
+    modifies ddbClient.Modifies, kmsClient.Modifies
+    ensures ddbClient.ValidState() && kmsClient.ValidState()
   {
-    res := Failure(E("Implement"));
+    var queryOutput :- QueryForActiveBranchKey(input.branchKeyIdentifier, ddbTableName, ddbClient);
+
+    :- Need(
+      //= aws-encryption-sdk-specification/framework/branch-key-store.md#versionkey
+      //= type=implication
+      //# The AWS DDB response MUST contain the fields defined in the [branch keystore record format](../#record-format).
+      //# If the record does not contain the defined fields, this operation MUST fail.
+      && validActiveBranchKey?(queryOutput.Items.value[0])
+      //= aws-encryption-sdk-specification/framework/branch-key-store.md#versionkey
+      //= type=implication
+      //# If the `type` on the item is not prefixed by "version", this operation MUST fail.
+      && queryOutput.Items.value[0][TYPE_FIELD].S[..|BRANCH_KEY_TYPE_PREFIX|] == BRANCH_KEY_TYPE_PREFIX,
+      Types.KeyStoreException(message := "Active key for " + input.branchKeyIdentifier + " does not have required fields.")
+    );
+    
+    var grantTokens := GetValidGrantTokens(input.grantTokens);
+    :- Need(
+      && grantTokens.Success?,
+      E("CreateKey received invalid grant tokens")
+    );
+
+    var item := queryOutput.Items.value[0];
+    
+    :- Need(
+      item[KMS_FIELD].S == kmsKeyArn,
+      Types.KeyStoreException(message := "Configured AWS KMS Key ARN does not match KMS Key ARN for branch-key-id: " + item[BRANCH_KEY_IDENTIFIER_FIELD].S)
+    );
+    
+
+    //= aws-encryption-sdk-specification/framework/branch-key-store.md#aws-kms-branch-key-reencryption
+    //= type=implication
+    //# The operation MUST create a branch key [encryption context](./structures.md#encryption-context)
+    //# from the branch AWS DDB query response according to [branch key encryption context](#encryption-context).
+    var oldActiveBranchKeyEncryptionContext := activeBranchKeyEncryptionContext(
+      item[KEY_IDENTIFIER_FIELD].S,
+      item[TYPE_FIELD].S[|BRANCH_KEY_TYPE_PREFIX|..],
+      item[KEY_CREATE_TIME].S,
+      ddbTableName,
+      item[KMS_FIELD].S
+    );
+    
+    //= aws-encryption-sdk-specification/framework/branch-key-store.md#aws-kms-branch-key-reencryption
+    //= type=implication
+    //# The operation MUST create a branch key [encryption context](./structures.md#encryption-context)
+    //# for DECRYPT_ONLY branch keys according to the [decrypt only branch key encryption context](#decrypt_only-encryption-context).
+    var decryptOnlyBranchKeyEncryptionContext: BranchKeyContext := decryptOnlyBranchKeyEncryptionContext(
+      item[KEY_IDENTIFIER_FIELD].S,
+      item[TYPE_FIELD].S[|BRANCH_KEY_TYPE_PREFIX|..],
+      item[KEY_CREATE_TIME].S,
+      ddbTableName,
+      item[KMS_FIELD].S
+    );
+
+    var decryptOnlyBranchKey :- ReEncryptBranchKeyDecryptOnly(
+      item[KEY_FIELD].B,
+      oldActiveBranchKeyEncryptionContext,
+      decryptOnlyBranchKeyEncryptionContext,
+      kmsKeyArn,
+      grantTokens.value,
+      kmsClient
+    );
+
+    //= aws-encryption-sdk-specification/framework/branch-key-store.md#versionkey
+    //# To create a new `ACTIVE` branch key under the supplied `branch-key-id` the operation
+    //# MUST generate the following values:
+
+
+    var maybeBranchKeyVersion := UUID.GenerateUUID();
+    //= aws-encryption-sdk-specification/framework/branch-key-store.md#versionkey
+    //# - `version`: a new guid. This guid MUST be [version 4 UUID](https://www.ietf.org/rfc/rfc4122.txt)
+    var branchKeyVersion :- maybeBranchKeyVersion
+      .MapFailure(e => Types.KeyStoreException(message := e));
+    //= aws-encryption-sdk-specification/framework/branch-key-store.md#versionkey
+    //# - `timestamp`: a timestamp for the current time. 
+    //# This MUST be in ISO8601 format in UTC, to microsecond precision (e.g. “YYYY-MM-DDTHH:mm:ss.ssssssZ“)
+    var timestamp :- Time.GetCurrentTimeStamp()
+      .MapFailure(e => E(e));
+    
+    var newActiveBranchKeyEncryptionContext: BranchKeyContext := activeBranchKeyEncryptionContext(
+      item[KEY_IDENTIFIER_FIELD].S,
+      branchKeyVersion,
+      timestamp,
+      ddbTableName,
+      kmsKeyArn 
+    );
+
+    var newBranchKeyWithoutPlaintext :- GenerateKey(
+      newActiveBranchKeyEncryptionContext,
+      kmsKeyArn,
+      grantTokens.value,
+      kmsClient
+    );
+
+    var decryptOnlyBranchKeyDDBMap := ToBranchKeyItemAttributeMap(decryptOnlyBranchKeyEncryptionContext, decryptOnlyBranchKey.CiphertextBlob.value);
+    var newActiveBranchKeyDDBMap := ToBranchKeyItemAttributeMap(newActiveBranchKeyEncryptionContext, newBranchKeyWithoutPlaintext.CiphertextBlob.value); 
+
+    var writeRotatedMaterials :- WriteVersionedKeyToStore(
+      decryptOnlyBranchKeyDDBMap,
+      newActiveBranchKeyDDBMap,
+      ddbTableName,
+      ddbClient 
+    );
+
+    res := Success(());
+  }
+
+  method QueryForActiveBranchKey(branchKeyId: string, ddbTableName: DDB.TableName, ddbClient: DDB.IDynamoDBClient)
+    returns (res: Result<DDB.QueryOutput, Types.Error>)
+    requires ddbClient.ValidState()
+    modifies ddbClient.Modifies
+    ensures ddbClient.ValidState()
+    ensures 
+      && |ddbClient.History.Query| > 0
+      && var ddbOperationInput := Last(ddbClient.History.Query).input;
+      && var ddbOperationOutput := Last(ddbClient.History.Query).output;
+      && ddbOperationOutput.Success?
+      && ddbOperationOutput.value.Items.Some?
+      //= aws-encryption-sdk-specification/framework/branch-key-store.md#versionkey
+      //= type=implication
+      //# There MUST only be one `ACTIVE` key. If there is more than one `ACTIVE` key, the operation MUST fail.
+      && |ddbOperationOutput.value.Items.value| > 1
+      ==> res.Failure?
+    ensures 
+      && |ddbClient.History.Query| > 0
+      && var ddbOperationOutput := Last(ddbClient.History.Query).output;
+      //= aws-encryption-sdk-specification/framework/branch-key-store.md#versionkey
+      //= type=implication
+      //# 1. If the client is unable to fetch an `ACTIVE` key, GetActiveBranchKey MUST fail.
+      && ddbOperationOutput.Failure?
+      ==> res.Failure?
+    ensures res.Success? ==>
+      && |ddbClient.History.Query| > 0
+      //= aws-encryption-sdk-specification/framework/branch-key-store.md#versionkey
+      //= type=implication
+      //# This operation MUST make a DDB::Query to get the branch key at `branchKeyId` with status `ACTIVE`
+      && var ddbOperationInput := Last(ddbClient.History.Query).input;
+      && var ddbOperationOutput := Last(ddbClient.History.Query).output;
+      && var expressionAttributeValues: DDB.AttributeMap := map[
+        EXPRESSION_ATTRIBUTE_VALUE_BRANCH_KEY := DDB.AttributeValue.S(branchKeyId),
+        EXPRESSION_ATTRIBUTE_VALUE_STATUS_KEY := DDB.AttributeValue.S(STATUS_ACTIVE)];
+      && ddbOperationOutput.Success?
+      && ddbOperationInput.TableName == ddbTableName
+      && ddbOperationInput.IndexName.Some?
+      && ddbOperationInput.IndexName.value == CreateKeyStoreTable.GSI_NAME
+      && ddbOperationInput.KeyConditionExpression.Some?
+      && ddbOperationInput.KeyConditionExpression.value == STATUS_BRANCH_KEY_ID_MATCH_EXPRESSION
+      && ddbOperationInput.ExpressionAttributeNames.Some?
+      && ddbOperationInput.ExpressionAttributeNames.value == EXPRESSION_ATTRIBUTE_NAMES
+      && ddbOperationInput.ExpressionAttributeValues.Some?
+      && ddbOperationInput.ExpressionAttributeValues.value == expressionAttributeValues
+      && ddbOperationOutput.value == res.value
+    ensures res.Success?
+      ==>
+        && res.value.Items.Some?
+        && |res.value.Items.value| == 1
+  {
+    var expressionAttributeValues : DDB.AttributeMap := map[
+      EXPRESSION_ATTRIBUTE_VALUE_BRANCH_KEY := DDB.AttributeValue.S(branchKeyId),
+      EXPRESSION_ATTRIBUTE_VALUE_STATUS_KEY := DDB.AttributeValue.S(STATUS_ACTIVE)
+    ];
+    
+    var queryInput := DDB.QueryInput(
+      TableName := ddbTableName,
+      IndexName := Some(CreateKeyStoreTable.GSI_NAME),
+      Select := None,
+      AttributesToGet := None,
+      Limit := None,
+      ConsistentRead :=  None,
+      KeyConditions := None,
+      QueryFilter := None,
+      ConditionalOperator := None,
+      ScanIndexForward := None,
+      ExclusiveStartKey := None,
+      ReturnConsumedCapacity :=  None,
+      ProjectionExpression := None,
+      FilterExpression := None,
+      KeyConditionExpression := Some(STATUS_BRANCH_KEY_ID_MATCH_EXPRESSION),
+      ExpressionAttributeNames := Some(EXPRESSION_ATTRIBUTE_NAMES),
+      ExpressionAttributeValues := Some(expressionAttributeValues)
+    );
+    
+    var maybeQueryResponse := ddbClient.Query(queryInput);
+    var queryResponse :- maybeQueryResponse
+      .MapFailure(e => Types.ComAmazonawsDynamodb(ComAmazonawsDynamodb := e));
+
+    :- Need(
+      && queryResponse.Items.Some?
+      && |queryResponse.Items.value| == 1,
+      E("Found more than one active key under: " + branchKeyId + ". Resolve by calling ActiveKeyResolution API.")
+    );
+
+    return Success(queryResponse);
+  }
+
+  method ReEncryptBranchKeyDecryptOnly(
+    ciphertext: seq<uint8>,
+    oldEncryptionContext: map<string, string>,
+    decryptOnlyEncryptionContext: map<string, string>,
+    awsKmsKey: KMS.KeyIdType,
+    grantTokens: KMS.GrantTokenList,
+    kmsClient: KMS.IKMSClient
+  )
+    returns (res: Result<KMS.ReEncryptResponse, Types.Error>)
+    requires kmsClient.ValidState()
+    requires KMS.IsValid_CiphertextType(ciphertext)
+    modifies kmsClient.Modifies
+    ensures kmsClient.ValidState()
+    ensures res.Success? ==>
+      && res.value.CiphertextBlob.Some?
+      && res.value.SourceKeyId.Some?
+      && res.value.KeyId.Some?
+      && res.value.SourceKeyId.value == awsKmsKey
+      && res.value.KeyId.value == awsKmsKey
+      //= aws-encryption-sdk-specification/framework/branch-key-store.md#aws-kms-branch-key-reencryption
+      //= type=implication
+      //# The operation MUST use the configured `KMS SDK Client` to decrypt the value of the branch key field.
+      && |kmsClient.History.ReEncrypt| > 0
+      && KMS.IsValid_CiphertextType(res.value.CiphertextBlob.value)
+      && var kmsOperationInput := Last(kmsClient.History.ReEncrypt).input;
+      && var kmsOperationOutput := Last(kmsClient.History.ReEncrypt).output;
+      && kmsOperationOutput.Success?
+      //= aws-encryption-sdk-specification/framework/branch-key-store.md#aws-kms-branch-key-reencryption
+      //= type=implication
+      //# When calling [AWS KMS API ReEncrypt](https://docs.aws.amazon.com/kms/latest/APIReference/API_ReEncrypt.html), 
+      //# the key store operation MUST call with a request constructed as follows:
+      && KMS.ReEncryptRequest(
+        //= aws-encryption-sdk-specification/framework/branch-key-store.md#aws-kms-branch-key-reencryption
+        //= type=implication
+        //# - `CiphertextBlob` MUST be the encrypted branch key value that is stored in AWS DDB.
+        CiphertextBlob := ciphertext,
+        //= aws-encryption-sdk-specification/framework/branch-key-store.md#aws-kms-branch-key-reencryption
+        //= type=implication
+        //# - `SourceEncryptionContext` MUST be the branch key encryption context.
+        SourceEncryptionContext := Some(oldEncryptionContext),
+        //= aws-encryption-sdk-specification/framework/branch-key-store.md#aws-kms-branch-key-reencryption
+        //= type=implication
+        //# - `SourceKeyId` MUST be the AWS KMS Key ARN configured in the key store operation.
+        SourceKeyId := Some(awsKmsKey),
+        //= aws-encryption-sdk-specification/framework/branch-key-store.md#aws-kms-branch-key-reencryption
+        //= type=implication
+        //# - `DestinationKeyId` MUST be the AWS KMS Key ARN configured in the key store operation.
+        DestinationKeyId := awsKmsKey,
+        //= aws-encryption-sdk-specification/framework/branch-key-store.md#aws-kms-branch-key-reencryption
+        //= type=implication
+        //# - `DestinationEncryptionContext` MUST be the DECRYPT_ONLY branch key encryption context created.
+        DestinationEncryptionContext := Some(decryptOnlyEncryptionContext),
+        SourceEncryptionAlgorithm := None,
+        DestinationEncryptionAlgorithm := None,
+        //= aws-encryption-sdk-specification/framework/branch-key-store.md#aws-kms-branch-key-reencryption
+        //= type=implication
+        //# - `GrantTokens` MUST be the [grant tokens](https://docs.aws.amazon.com/kms/latest/developerguide/concepts.html#grant_token)
+        GrantTokens := Some(grantTokens)
+      ) == kmsOperationInput
+      && kmsOperationOutput.value.CiphertextBlob.Some?
+      && kmsOperationOutput.value.SourceKeyId.Some?
+      && kmsOperationOutput.value.KeyId.Some?
+      && kmsOperationOutput.value.CiphertextBlob.value == res.value.CiphertextBlob.value
+      && kmsOperationOutput.value.SourceKeyId.value == res.value.SourceKeyId.value
+      && kmsOperationOutput.value.KeyId.value == res.value.KeyId.value
+  {
+    var reEncryptRequest := KMS.ReEncryptRequest(
+      CiphertextBlob := ciphertext,
+      SourceEncryptionContext := Some(oldEncryptionContext),
+      SourceKeyId := Some(awsKmsKey),
+      DestinationKeyId := awsKmsKey,
+      DestinationEncryptionContext := Some(decryptOnlyEncryptionContext),
+      SourceEncryptionAlgorithm := None,
+      DestinationEncryptionAlgorithm := None,
+      GrantTokens := Some(grantTokens)
+    );
+
+    var maybeReEncryptResponse := kmsClient.ReEncrypt(reEncryptRequest);
+    var reEncryptResponse :- maybeReEncryptResponse
+      .MapFailure(e => Types.ComAmazonawsKms(ComAmazonawsKms := e));
+    
+    :- Need(
+      && reEncryptResponse.SourceKeyId.Some?
+      && reEncryptResponse.KeyId.Some?
+      && reEncryptResponse.SourceKeyId.value == awsKmsKey
+      && reEncryptResponse.KeyId.value == awsKmsKey 
+      && ParseAwsKmsIdentifier(reEncryptResponse.SourceKeyId.value).Success?
+      && ParseAwsKmsIdentifier(reEncryptResponse.KeyId.value).Success?,
+      Types.KeyStoreException(
+        message := "Invalid response from KMS GenerateDataKey:: Invalid Key Id")
+    );
+
+    :- Need(
+      && reEncryptResponse.CiphertextBlob.Some?
+      && KMS.IsValid_CiphertextType(reEncryptResponse.CiphertextBlob.value),
+      Types.KeyStoreException(
+        message := "Invalid response from AWS KMS GeneratedDataKey: Invalid ciphertext")
+    );
+
+    return Success(reEncryptResponse);
   }
 }
